First attempts to add Security.thy and combine with Capture

Security.thy
@@ -5,6 +5,7 @@ begin
 locale security = rules 
 
 type_synonym ('a,'b) Trace = "('b \<times> 'b) set list" 
+type_synonym ('a,'b) LTrace = "('b set \<times> ('b \<times> 'b) set) list" 
 
 context security
 begin
@@ -26,11 +27,26 @@ definition ev :: "('a,'b) com \<Rightarrow> 'b \<Rightarrow> ('a,'b) Trace \<Rig
   ("\<langle>_,_\<rangle> \<rightarrow>\<^sup>*_ \<langle>_,_\<rangle>" [50,40,40] 70)
   where "\<langle>c,m\<rangle> \<rightarrow>\<^sup>*t \<langle>c',m'\<rangle> \<equiv> trace_mem m t m' \<and> c \<mapsto>\<^sup>*t c'"
 
+text \<open> trace as list of local steps in order to collect vc + beh \<close>
+
+inductive_set local_trace :: "(('a,'b) com \<times> ('a,'b) LTrace \<times> ('a,'b) com) set"
+  and local_trace_abv :: "('a,'b) com \<Rightarrow> ('a,'b) LTrace \<Rightarrow> ('a,'b) com \<Rightarrow> bool" 
+                                                                       ("_ \<mapsto>\<^sup>l\<^sup>*_ _" [50,40,40] 70)
+  where
+  "local_trace_abv P t P' \<equiv> (P, t, P') \<in> local_trace"
+  | none[intro]: "c \<mapsto>\<^sup>l\<^sup>*[] c" 
+  | sil[intro]: "c\<^sub>1 \<leadsto> c\<^sub>2 \<Longrightarrow> c\<^sub>2 \<mapsto>\<^sup>l\<^sup>*t c\<^sub>3 \<Longrightarrow> c\<^sub>1 \<mapsto>\<^sup>l\<^sup>*t c\<^sub>3"
+  | gex[intro]: "c\<^sub>1 \<mapsto>[\<alpha>',r,\<alpha>] c\<^sub>2 \<Longrightarrow> c\<^sub>2 \<mapsto>\<^sup>l\<^sup>*t c\<^sub>3 \<Longrightarrow> c\<^sub>1 \<mapsto>\<^sup>l\<^sup>*(strip_tag \<alpha>')#t c\<^sub>3"
+
+
 (*non-interference over all basic commands *)
+definition tag_basic
+  where "tag_basic a \<alpha> \<equiv>  (tag a, \<alpha>)"
 
 definition sec_pres :: "('a,'b) com \<Rightarrow> 'b rel \<Rightarrow> bool"
-  where "sec_pres c S \<equiv> \<forall>\<alpha> r m\<^sub>1 m\<^sub>2 m\<^sub>1'. \<alpha> \<in> basics c \<longrightarrow> m\<^sub>1 \<in> vc \<alpha>\<llangle>r\<rrangle> \<longrightarrow> (m\<^sub>1,m\<^sub>2) \<in> S \<longrightarrow> 
-                             (m\<^sub>1,m\<^sub>1') \<in> beh \<alpha>\<llangle>r\<rrangle> \<longrightarrow> (\<exists>m\<^sub>2'. (m\<^sub>2,m\<^sub>2') \<in> beh \<alpha>\<llangle>r\<rrangle> \<and> (m\<^sub>1',m\<^sub>2') \<in> S)"
+  where "sec_pres c S \<equiv> \<forall>\<alpha> r m\<^sub>1 m\<^sub>2 m\<^sub>1'. (strip_tag \<alpha>) \<in> obs_basics c \<longrightarrow> 
+                m\<^sub>1 \<in> (vc \<alpha>\<llangle>r\<rrangle>) \<longrightarrow> (m\<^sub>1,m\<^sub>2) \<in> S \<longrightarrow> (m\<^sub>1,m\<^sub>1') \<in> beh \<alpha>\<llangle>r\<rrangle> \<longrightarrow> 
+                               (\<exists>m\<^sub>2'. (m\<^sub>2,m\<^sub>2') \<in> beh \<alpha>\<llangle>r\<rrangle> \<and> (m\<^sub>1',m\<^sub>2') \<in> S)"
 
 (* non-interference over all traces *)
 
@@ -59,10 +75,114 @@ lemma trace_preE [elim]:
   obtains P\<^sub>2 where "P\<^sub>1 \<mapsto>\<^sup>*[x] P\<^sub>2" "P\<^sub>2 \<mapsto>\<^sup>*t P\<^sub>3"
   using assms by (metis append.simps(1) append.simps(2) trace_concatE)
 
+lemma basics_exec_step:
+  assumes "c \<mapsto>[\<alpha>'',r,\<alpha>] c'" 
+  shows "\<alpha> \<in> basics c"
+  using assms by induct auto
+
+(*
+lemma obs_basics_silent: 
+  assumes "P\<^sub>1 \<leadsto> P\<^sub>2"
+  shows "obs_basics P\<^sub>1 \<supseteq> obs_basics P\<^sub>2"
+  using assms basics_exec 
+proof (induct)
+  case (capS c c' k)
+  then show ?case
+    apply simp 
+    by blast
+next
+  case (capStep c \<alpha>' r \<alpha> c' s s')
+  have \<alpha>: "\<alpha>' = \<alpha>\<llangle>r\<rrangle>" using capStep lexecute_triple by auto
+  hence " basics c' \<subseteq>  basics c" using capStep by auto
+  hence " obs_basics c' \<subseteq>  obs_basics c" using capStep sledgehammer
+  hence "\<Union> (observable ` basics c') \<subseteq> \<Union> (observable ` basics c)" 
+  moreover have "\<exists>x\<in>basics c. popbasic' s s' \<alpha>' \<in> observable x"
+    unfolding overapprox_def 
+      
+      sorry
+  ultimately show ?case by simp
+qed auto
+*)
+
+
+(*
+
+lemma helpCap: 
+  assumes  "c \<mapsto>[\<alpha>',r,\<alpha>] c'" 
+  assumes  "c \<mapsto>[\<alpha>',r,\<alpha>] c' \<Longrightarrow> basics c' \<subseteq> basics c"
+  shows "obs_basics (Basic (popbasic' s s' \<alpha>') \<cdot> Capture s' c') \<subseteq> obs_basics (Capture s c)" 
+  using assms apply auto
+proof -
+  have a0:"\<exists>x\<in>obs_basics c. (poppred' s (vc \<alpha>'), poprel' s s' (beh \<alpha>')) \<in> observable x"
+  
+
+     sorry
+
+(*
+"\<exists>x\<in>obs_basics c. (poppred' s (vc \<alpha>'), poprel' s s' (beh \<alpha>')) \<in> observable x"
+"\<And>a b aa ba. (aa, ba) \<in> obs_basics c' \<Longrightarrow> (a, b) \<in> observable (aa, ba) \<Longrightarrow> 
+                                           \<exists>x\<in>obs_basics c. (a, b) \<in> observable x"
+*)
+
+
+lemma helpS: 
+  assumes "s \<in> S"
+  shows  "obs_basics (seq2com s) \<subseteq> (\<Union>s\<in>S. strip_tag_set (set s))"
+  sorry
+
+
+lemma basics_silent:
+  assumes "c \<leadsto> c'"
+  shows "obs_basics c \<supseteq> obs_basics c'"
+  using assms basics_exec 
+proof (induct)
+next 
+  case (bigc s S)
+  then show ?case by (simp add: helpS) 
+next
+  case (capS c c' k)
+  then show ?case apply simp by blast
+next
+  case (capStep c \<alpha>' r \<alpha> c' s s')
+  have a0: "\<alpha>' = \<alpha>\<llangle>r\<rrangle>" using capStep lexecute_triple by auto
+  hence a1: "basics c' \<subseteq>  basics c" using capStep by auto
+(*  have a2: "popbasic' s s' \<alpha>' \<in> popbasic ` basics c" sorry
+  have a3: "popbasic ` basics c' \<subseteq> popbasic ` basics c" sorry  *)
+  show ?case using helpCap using capStep.hyps using a1 by presburger
+qed auto
+*)
+
+text \<open>Identify all observable operations in a trace\<close>
+
+definition obs_atomics :: "('a,'b) com \<Rightarrow> ('b set \<times> 'b rel) set" 
+  where "obs_atomics c \<equiv> { \<alpha> | \<alpha> t c' . c \<mapsto>\<^sup>l\<^sup>*t c' \<and> \<alpha> \<in> set t }"
+
+
+definition obs_atomics' :: "('a,'b) com \<Rightarrow> ('b set \<times> 'b rel) set" 
+  where "obs_atomics c \<equiv> { \<alpha> | \<alpha> t c' . c \<mapsto>\<^sup>*t c' \<and> \<alpha> \<in> reorder_trace t c }"
+
+
+
+lemma basics_silent:
+  assumes "c \<leadsto> c'"
+  shows "obs_atomics c \<supseteq> obs_atomics c'"  sorry
+
+
+
+lemma obs_basics_lexec:
+  assumes "lexecute c \<alpha>' r \<alpha> c'" 
+  shows "obs_basics c \<supseteq> obs_basics c'"
+  using assms by (induct) auto
+
+lemma obs_basics_gex: 
+  assumes "gexecute c g c'" shows "obs_basics c \<supseteq> obs_basics c'"
+  using assms obs_basics_lexec by (induct) auto 
+
+
 lemma trace_basics: 
   assumes "P\<^sub>1 \<mapsto>\<^sup>*t P\<^sub>2"
-  shows "basics P\<^sub>1 \<supseteq> basics P\<^sub>2"
-  using assms basics_silent basics_gex by induct blast+
+  shows "obs_basics P\<^sub>1 \<supseteq> obs_basics P\<^sub>2"
+  using assms basics_silent obs_basics_gex by induct blast+
 
 lemma basic_par_subset: (*Nick help with name please*)
   assumes "gexecute c g c'" 
@@ -70,13 +190,13 @@ lemma basic_par_subset: (*Nick help with name please*)
         "basics c\<^sub>2 \<subseteq> basics (c\<^sub>1 || c\<^sub>2)" 
   using assms by simp+
 
+(* ---not used:
 lemma something1: (*Nick help with name please*)
   assumes "gexecute c g c'" 
   shows "\<exists>r \<alpha>. \<alpha> \<in> basics c \<and> g = beh \<alpha>\<llangle>r\<rrangle>"
   using assms proof induct
   case (thr c r \<alpha> c')
-  then show ?case using basics.simps(8) basics_lexec_prefix 
-  by (metis insert_subset lexecute_triple)
+  then show ?case using basics.simps(8) basics_lexec_prefix by blast
 qed auto
 
 lemma something2: (*Nick help with name please*)
@@ -90,6 +210,8 @@ next
   case (gex c\<^sub>1 c\<^sub>2 c\<^sub>3)
   then show ?case using something1 by force
 qed
+*)
+
 
 lemma trace_rule_nil: 
   assumes "c \<mapsto>\<^sup>*[] c'"
@@ -100,7 +222,7 @@ lemma trace_rule_nil:
 lemma trace_rule: 
   assumes "c \<mapsto>\<^sup>*[g] c'"
   assumes "R,G \<turnstile> P {c} Q"
-  shows "\<exists>\<alpha> r M. \<alpha> \<in> basics c \<and> g = beh \<alpha>\<llangle>r\<rrangle> \<and> P \<subseteq> wp\<^sub>\<alpha> \<alpha>\<llangle>r\<rrangle> M \<and> guar\<^sub>\<alpha> \<alpha>\<llangle>r\<rrangle>  G \<and> R,G \<turnstile> M {c'} Q"
+  shows "\<exists>\<alpha> r M. (strip_tag \<alpha>) \<in> obs_basics c \<and> g = beh \<alpha>\<llangle>r\<rrangle> \<and> P \<subseteq> wp\<^sub>\<alpha> \<alpha>\<llangle>r\<rrangle> M \<and> guar\<^sub>\<alpha> \<alpha>\<llangle>r\<rrangle>  G \<and> R,G \<turnstile> M {c'} Q"
   using assms 
 proof (induct c "[g]" c' arbitrary: P) 
   case (sil c\<^sub>1 c\<^sub>2 c\<^sub>3)
@@ -108,9 +230,7 @@ proof (induct c "[g]" c' arbitrary: P)
     by (metis (no_types, hide_lams) insert_subset subsetI subset_antisym)
 next
   case (gex c\<^sub>1 c\<^sub>2 c\<^sub>3)
-  then show ?case using trace_rule_nil gexecute_ruleI[OF gex(3,1)] 
-    sorry
-(*    by fast *)
+  then show ?case using trace_rule_nil gexecute_ruleI[OF gex(3,1)] sorry (*by fast *) 
 qed 
 
 lemma bisim_exists:
@@ -131,7 +251,7 @@ proof safe
   next
     case (2 m\<^sub>1 m\<^sub>1' g t m\<^sub>1'')
     then obtain c' where itm1: "c \<mapsto>\<^sup>*[g] c'" "c' \<mapsto>\<^sup>*t c\<^sub>1" by auto
-    then obtain P' r \<alpha> where itm2: "R,G \<turnstile> P' {c'} Q" "\<alpha> \<in> basics c" 
+    then obtain P' r \<alpha> where itm2: "R,G \<turnstile> P' {c'} Q" "(strip_tag \<alpha>) \<in> obs_basics c" 
       "g = beh \<alpha>\<llangle>r\<rrangle>" "P \<subseteq> wp\<^sub>\<alpha> \<alpha>\<llangle>r\<rrangle> P'"  using trace_rule[OF itm1(1) 2(5)] by blast
     hence itm6: "m\<^sub>1' \<in> P'" using 2(1,8) unfolding wp_def by blast                       
     then obtain m\<^sub>2' where itm3: "(m\<^sub>2,m\<^sub>2') \<in> g" "(m\<^sub>1',m\<^sub>2') \<in> S" using 2(1,4,6,8) itm2(2,3,4) 
